clean.sh
@@ -1,4 +1,10 @@
 pushd theorems
 make clean
-rm -f .*.vo.aux
+rm -f *.glob
+rm -f *.vo
+rm -f *.vok
+rm -f *.vos
+rm -f .*.aux
+rm -f .*.d
+rm -f Makefile*
 popd
