theorems/known_types.md
@@ -1,3 +1,217 @@
+```coq
+(*
+  okay I feel like I want to have a `compile` function that takes terms and just reduces the knowns, typechecks them, and outputs a string representing the "compiled" program
+  then a `run` function that reduces the knowns and typechecks the program, but then reduces all the terms and outputs the "stdout" of the program
+  this is presupposing that you'll have some kind of effectful commands that append some string to the "stdout". that seems like the more natural way I would prefer to structure a language that I'll eventually be using to learn while making a real imperative language
+*)
+
+(*Require Import Coq.Strings.String.
+Require Import theorems.Maps.
+
+Inductive typ: Type :=
+  (*| Generic*)
+  | Bool
+  | Nat
+  | Arrow (input output: typ)
+  | UnionNil
+  | UnionCons (arm_name: string) (arm_type: typ) (rest: typ)
+  | TupleNil
+  | TupleCons (left right: typ)
+  (*| KnownType (type_value: trm)*)
+  (*| KnownValue (value: trm)*)
+.
+
+Inductive Arm: Type :=
+  | arm (arm_name: string).
+
+Inductive trm: Type :=
+  | tru | fls
+  | debug_bool
+  (*| nat_const (n: nat)*)
+  (*| nat_plus (left right: trm)*)
+  (*| debug_nat*)
+  | binding (decl_name: string) (after: trm)
+  | usage (var_name: string)
+  | test (conditional iftru iffls: trm)
+  | fn (args_name: string) (output_type: typ) (body: trm)
+  | call (target_fn args: trm)
+  | union_nil
+  | union_cons (arm_name: string) (arm_value: trm) (rest_type: typ)
+  | union_match (tr: trm) (arms: list (string * trm))
+  | tuple_nil
+  | tuple_cons (left right: trm)
+  | tuple_access (tup: trm) (index: nat)
+.
+
+
+Fixpoint tuple_lookup (n: nat) (tr: trm): option trm :=
+  match tr with
+  | tuple_cons t tr' => match n with
+    | 0 => Some t
+    | S n' => tuple_lookup n' tr'
+    end
+  | _ => None
+  end
+.
+
+Fixpoint union_lookup (tr: trm) (arms: list (string, (string * trm))): option trm :=
+  match tr with
+  | union_cons tr_arm_name tr_arm_value _ => match arms with
+    | (arm_name, (arm_var, arm_body)) :: arms' => if eqb_string tr_arm_name arm_name
+      then Some (substitute arm_var tr_arm_value arm_body)
+      else union_lookup tr arms'
+    | [] => None
+    end
+  | _ => None
+  end
+.
+*)
+
+
+
+
+
+
+(*Require Import Coq.Strings.String.
+Require Import theorems.Maps.
+
+(*Notation memarr := (@list string).*)
+
+
+Inductive typ: Type :=
+  | Base: string -> typ
+  | Arrow: typ -> typ -> typ
+  | TupleNil: typ
+  | TupleCons: typ -> typ -> typ.
+
+
+Inductive trm: Type :=
+  | var: string -> trm
+  | call: trm -> trm -> trm
+  | fn: string -> typ -> trm -> trm
+  (* tuples *)
+  | tuple_proj: trm -> nat -> trm
+  | tuple_nil: trm
+  | tuple_cons: trm -> trm -> trm.
+
+
+Inductive tuple_typ: typ -> Prop :=
+  | TTnil:
+    tuple_typ TupleNil
+  | TTcons: forall T1 T2,
+    tuple_typ (TupleCons T1 T2).
+
+Inductive well_formed_typ: typ -> Prop :=
+  | wfBase: forall i,
+    well_formed_typ (Base i)
+  | wfArrow: forall T1 T2,
+    well_formed_typ T1 ->
+    well_formed_typ T2 ->
+    well_formed_typ (Arrow T1 T2)
+  | wfTupleNil:
+    well_formed_typ TupleNil
+  | wfTupleCons: forall T1 T2,
+    well_formed_typ T1 ->
+    well_formed_typ T2 ->
+    tuple_typ T2 ->
+    well_formed_typ (TupleCons T1 T2).
+
+Hint Constructors tuple_typ well_formed_typ.
+
+Inductive tuple_trm: trm -> Prop :=
+  | tuple_tuple_nil:
+    tuple_trm tuple_nil
+  | tuple_trm_tuple_cons: forall t1 t2,
+    tuple_trm (tuple_cons t1 t2).
+
+Hint Constructors tuple_trm.
+
+(*Notation "x :: l" := (cons x l)
+                     (at level 60, right associativity).*)
+Notation "{ }" := tuple_nil.
+Notation "{ x ; .. ; y }" := (tuple_cons x .. (tuple_cons y tuple_nil) ..).
+
+
+Fixpoint subst (prev: string) (next: trm) (target: trm) : trm :=
+  match target with
+  | var y => if eqb_string prev y then next else target
+  | fn y T t1 => fn y T (if eqb_string prev y then t1 else (subst prev next t1))
+  | call t1 t2 => call (subst prev next t1) (subst prev next t2)
+  | tuple_proj t1 i => tuple_proj (subst prev next t1) i
+  | tuple_nil => tuple_nil
+  | tuple_cons t1 tup => tuple_cons (subst prev next t1) (subst prev next tup)
+  end.
+
+Notation "'[' prev ':=' next ']' target" := (subst prev next target) (at level 20).
+
+
+Inductive value: trm -> Prop :=
+  | v_fn: forall x T11 t12,
+    value (fn x T11 t12)
+  | v_tuple_nil: value tuple_nil
+  | v_tuple_cons: forall v1 vtup,
+    value v1 ->
+    value vtup ->
+    value (tuple_cons v1 vtup).
+
+Hint Constructors value.
+
+Fixpoint tuple_lookup (n: nat) (tr: trm): option trm :=
+  match tr with
+  | tuple_cons t tr' => match n with
+    | 0 => Some t
+    | S n' => tuple_lookup n' tr'
+    end
+  | _ => None
+  end.
+
+
+Open Scope string_scope.
+
+Notation a := (var "a").
+Notation b := (var "b").
+Notation c := (var "c").
+Notation d := (var "d").
+Notation e := (var "e").
+Notation f := (var "f").
+Notation g := (var "g").
+Notation l := (var "l").
+Notation A := (Base "A").
+Notation B := (Base "B").
+Notation k := (var "k").
+Notation i1 := (var "i1").
+Notation i2 := (var "i2").
+
+
+Example test_tuple_lookup_nil_0:
+  (tuple_lookup 0 {}) = None.
+Proof. reflexivity. Qed.
+
+Example test_tuple_lookup_nil_1:
+  (tuple_lookup 1 {}) = None.
+Proof. reflexivity. Qed.
+
+Example test_tuple_lookup_cons_valid_0_a:
+  (tuple_lookup 0 { a }) = Some a.
+Proof. reflexivity. Qed.
+
+Example test_tuple_lookup_cons_valid_0_a_b:
+  (tuple_lookup 0 { a; b }) = Some a.
+Proof. reflexivity. Qed.
+
+Example test_tuple_lookup_cons_invalid:
+  (tuple_lookup 3 { a; b; c }) = None.
+Proof. reflexivity. Qed.
+*)
+
+```
+
+
+
+
+
+
+
 You should probably write out this whole (almost) blog post informally before you really dig into the formal stuff. This is just such a huge undertaking, first understanding what you even precisely want to accomplish is a good idea.
 
 Think of it like writing the documentation before you write the code! You do that all the time since it helps clarify what's special and useful about the code, and what features it needs to have.
